examples/eip20/EIP20TokenPrinters.v
@@ -1,7 +1,7 @@
 From ConCert.Execution Require Import Blockchain.
 From ConCert.Execution Require Import Serializable.
 From ConCert.Execution.Test Require Import QCTest.
-From ConCert.Examples Require Import EIP20Token.
+From ConCert.Examples.EIP20 Require Import EIP20Token.
 
 Local Open Scope string_scope.
 
